**非递归： 思路很强**
```C++
class Solution {
public:
    vector<string> generateParenthesis(int n) {
        if (n == 0)
            return {};
        if (n == 1)
            return {"()"};
        vector<vector<string>> dp(n+1);
        dp[0] = {""};
        dp[1] = {"()"};
        for (int i = 2; i <= n; i++)
        {
            for (int j = 0; j < i; j++)
            {
                for (string p : dp[j])
                {
                    for (string q : dp[i - j - 1])
                    {
                        string str = "(" + p + ")" + q;
                        dp[i].push_back(str);
                    }
                }
            }
        }
        return dp[n];
    }
};
```

**递归**
```C++
class Solution {
public:
    vector<string> res;
    void dfs(int n, int lc, int rc, string path)
    {
        if (lc==n && rc==n)
            res.push_back(path);
        else
        {
            if (lc < n)
                dfs(n, lc + 1, rc, path + "(");
            if (rc < n && lc > rc)
                dfs(n, lc, rc + 1, path + ")");
        }
    }

    vector<string> generateParenthesis(int n) {
        dfs(n, 0, 0, "");
        return res;
    }
};
```